\documentclass[UTF8]{article}
\usepackage{amsmath}
\usepackage{amsfonts}
\usepackage{graphicx}
\usepackage[shortlabels]{enumitem}
\usepackage[T1]{fontenc}
\newenvironment{tightcenter}{%
  \setlength\topsep{0pt}
  \setlength\parskip{0pt}
  \begin{center}
}{%
  \end{center}
}
\setlength\topmargin{0pt}
\addtolength\topmargin{-\headheight}
\addtolength\topmargin{-\headsep}
\setlength\oddsidemargin{0pt}
\setlength\textwidth{\paperwidth}
\addtolength\textwidth{-2in}
\setlength\textheight{\paperheight}
\addtolength\textheight{-2in}
\usepackage{layout}
\setlength\parindent{6pt}
\begin{document}
\title{%
 \textbf{DSGE Problem Set WriteUp}  \\
 \large OSE Bootcamp 2019 Week 3 }
\author{Alan Shenkerman } 
\date{Monday, July 22, 2019}
\maketitle

\section*{DSGE Models}

\subsection*{Exercise 1}
We substitute $K_{t+1} = A e^{z_t} K_t^{\alpha}$ into each side of the Euler equation and find the correct value of $A$ in terms of the model parameters. Simplifying the LHS:
\begin{align*}
\frac{1}{e^{z_t}K_t^{\alpha} - K_{t+1}}  = \frac{1}{e^{z_t}K_t^{\alpha} - A e^{z_t} K_t^{\alpha}} = \frac{1}{e^{z_t} K_t^{\alpha} (1 - A)}
\end{align*}
On the RHS, note $E(z_{t+1}) = \rho z_t$. We get.
\begin{align*}
\beta E_t \left[ \frac{\alpha e^{z_{t +1}} K_{t+1}^{\alpha -1}}{ e^{z_{t +1}} K_{t+1}^{\alpha} - K_{t+2}}  \right]  &= \beta E_t \left[ \frac{\alpha e^{z_{t +1}} (A e^{z_t} K_t^{\alpha})^{\alpha -1}}{ e^{z_{t +1}} (A e^{z_t} K_t^{\alpha})^{\alpha} - Ae^{z_{t+1}} (Ae^{z_t} K_t^{\alpha})^{\alpha}}  \right]  \\
&= \frac{\alpha \beta}{Ae^{z_t}K_t^{\alpha}(1-A)}
\end{align*}
Combining the two, most terms cancel and we're left with 
$$A = \alpha \beta,$$ so our steady-state policy function becomes:
$$K_{t+1} = \alpha \beta e^{z_t} K_t^\alpha.$$

\subsection*{Exercise 2}
The characterizing equations are:
\begin{align*}
c_{t}&=(1-\tau)\left[w_{t} l_{t}+\left(r_{t}-\delta\right) k_{t}\right]+k_{t}+T_{t}-k_{t+1} \\
\frac{1}{c_{t}}&=\beta E\left\{\frac{1}{c_{t+1}}\left[(r_{t+1}-\sigma\right)(1-\tau)+1\right] \} \\
\frac{a}{1-l_{t}}&=\frac{1}{c_{t}} w_{t}(1-\tau) \\
r_{t}&=\alpha e^{z_{t}} k_{t}^{\alpha-1} l_{t}^{1-\alpha} \\ 
w_{t}&=(1-\alpha) e^{z_t} k_{t}^{\alpha} l_{t}^{-\alpha} \\
T_t &= \tau\left[w_{t} l_{t}+\left(r_{t}-\delta\right) k_{t}\right] \\
z_{t}&=\left(1-\rho_{z}\right) \overline{z}+\rho_{z} z_{t-1}+\epsilon_{t}^{z}
\end{align*}
Note since here we have to consider leisure as well as consumption, the policy function is more complex and the simple form from Exercise 1 will not hold. 

\subsection*{Exercise 3}
The characterizing equations are:
\begin{align*}
c_{t}&=(1-\tau)\left[w_{t} l_{t}+\left(r_{t}-\delta\right) k_{t}\right]+k_{t}+T_{t}-k_{t+1} \\
c_{t}^{-\gamma}&=\beta E_t\left\{c_{t+1}^{-\gamma}\left[\left(r_{t+1}-\delta\right)(1-\tau)+1\right]\right\} \\
\frac{a}{1-l_{t}}&=c_{t}^{-\gamma} w_{t}(1-\tau) \\
r_{t}&=\alpha e^{z_{t}} k_{t}^{\alpha-1} l_{t}^{1-\alpha} \\
w_{t}&=(1-\alpha)e^{z_{t}} k_{t}^{\alpha} l_{t}^{-\alpha} \\
T_t &= \tau\left[w_{t} l_{t}+\left(r_{t}-\delta\right) k_{t}\right] \\
z_{t}&=\left(1-\rho_{z}\right) \overline{z}+\rho_{z} z_{t-1}+\epsilon_{t}^{z}
\end{align*}

\subsection*{Exercise 4}
The characterizing equations are:
\begin{align*}
c_{t}&=(1-\tau)\left[w_{t} l_{t}+\left(r_{t}-\delta\right) k_{t}\right]+k_{t}+T_{t}-k_{t+1} \\
c_{t}^{-\gamma}&=\beta E_{t}\left\{c_{t+1}^{-\gamma}\left[\left(r_{t+1}-\delta\right)(1-\tau)+1\right]\right\} \\
a\left(1-l_{t}\right)^{-\xi}&=c_{t}^{-\gamma} w_{t}(1-\tau) \\
r_t &= \alpha e^{z_t} k_t^{\eta - 1} [\alpha k_t^{\eta} + (1 - \alpha) l_t^{\eta}]^{\frac{1 - \eta}{\eta}} \\
w_t &= (1 - \alpha) e^{z_t} l_t^{\eta - 1} [\alpha k_t^{\eta} + (1 - \alpha) l_t^{\eta}]^{\frac{1 - \eta}{\eta}} \\
	 T_t &= \tau[w_tl_t + (r_t - \delta)k_t] \\
	z_t &= (1-\rho_z)\bar{z} + \rho_z z_{t-1} + \epsilon^z_t
\end{align*}

\subsection*{Exercise 5}
Characterizing Equations, $l_t = 1$: 
\begin{align*}
c_{t}&=(1-\tau)\left[w_{t}+\left(r_{t}-\delta\right) k_{t}\right]+k_{t}+T_{t}-k_{t+1} \\
c_{t}^{-\gamma}&=\beta E_t\left\{c_{t+1}^{-\gamma}\left[\left(r_{t+1}-\delta\right)(1-\tau)+1\right]\right\} \\
r_{t}&=\alpha e^{z_{t}} k_{t}^{\alpha-1} e^{z_t(1-\alpha)} \\
w_{t}&=(1-\alpha)e^{z_{t}(1-\alpha} k_{t}^{\alpha}\\
T_t &= \tau\left[w_{t} +\left(r_{t}-\delta\right) k_{t}\right] \\
z_{t}&=\left(1-\rho_{z}\right) \overline{z}+\rho_{z} z_{t-1}+\epsilon_{t}^{z}
\end{align*}
It follows that the steady state versions are:
\begin{align*}
	\bar{c} &= (1 - \tau)[\bar{w}+ (\bar{r} - \delta) \bar{k}] + \bar{k} + \bar{T} - \bar{k} \\
	\bar{T} &= \tau [\bar{w} + (\bar{r}- \delta)\bar{k} ] \\
	\bar{c} ^{-\gamma} &= \beta E_t \left[ \bar{c}^{-\gamma} [(\bar{r} - \delta)(1 - \tau) + 1] \right] \\
	\bar{r} &= \alpha \bar{k} ^{\alpha - 1} (e^{\bar{z}})^{1 - \alpha} \\
	\bar{w} &= (1 - \alpha) \bar{k} ^{\alpha} (e^{\bar{z}})^{1 - \alpha} \\
	\bar{z} &= (1 - \rho_z)\bar{z} + \rho_z \bar{z}
\end{align*}
We solve these analytically for $\bar{K}$ as a function of the parameters of the model to see that:
$$\bar{K} = e^{\bar{z}}  \sqrt[1-\alpha]{\frac{\alpha}{\delta + \frac{1-\beta}{\beta (1-\tau)}}}.$$ We see in our Jupyter Notebook that this coincides with very high accuracy to the numerical steady state solution. 

\subsection*{Exercise 6}
Characterizing Equations:
\begin{align*}
	c_t &= (1 - \tau)[w_tl_t + (r_t -\delta)k_t] + k_t + T_t - k_{t+1} \\
	c_t ^{-\gamma} &= \beta E_t\left[ c_{t+1}^{-\gamma} [(r_{t+1} - \delta)(1 - \tau) + 1]\right] \\
	\frac{a}{(1-l_t)^{\xi}} &= c_t ^{-\gamma} w_t (1-\tau) \\
	r_t &= \alpha \left( \frac{l_t e^{z_t}}{k_t} \right)^{1 - \alpha} \\
	w_t &= (1 - \alpha) e^{z_t} \left( \frac{k_t}{l_t e^{z_t}} \right)^{\alpha} \\
	 T_t &= \tau[w_tl_t + (r_t - \delta)k_t] \\
	z_t &= (1-\rho_z)\bar{z} + \rho_z z_{t-1} + \epsilon^z_t; \quad \epsilon^z_t \sim i.i.d. (0, \sigma^2_z)
\end{align*}

Steady State:
\begin{align*}
	\bar{c} &= (1 - \tau)[\bar{w} \bar{l} + (\bar{r} -\delta)\bar{k}] + \bar{k} + \bar{T} - \bar{k} \\
	\bar{c} ^{-\gamma} &= \beta E_t\left[ \bar{c}^{-\gamma} [(\bar{r} - \delta)(1 - \tau) + 1]\right] \\
	\frac{a}{(1-\bar{l})^{\xi}} &= \bar{c} \bar{w} (1-\tau) \\
	\bar{r} &= \alpha \left( \frac{\bar{l} e^{\bar{z}}}{\bar{k}} \right)^{1 - \alpha} \\
	\bar{w} &= (1 - \alpha) e^{\bar{z}} \left( \frac{\bar{k}}{\bar{l} e^{\bar{z}}} \right)^{\alpha} \\
	 \bar{T} &= \tau[\bar{w} \bar{l} + (\bar{r} - \delta)\bar{k}] \\
	\bar{z} &= (1-\rho_z)\bar{z} + \rho_z \bar{z} 
\end{align*}


\section*{Linearization Methods}

\subsection*{Exercise 3}
We simplify:
\begin{align*}
&E_t\{FX_{t+1} + GX_t + HX_{t-1} + LZ_{t+1} + MZ_t\} \\
&E_t\{F(PX_t + Z_{t+1}) + G(PX_{t-1} + QZ_t) + HX_{t-1} + L(NZ_t + \epsilon_{t+1}) + MZ_t\} \\
&E_t\{F(P(PX_{t-1} + QZ_{t+1}) + NZ_t + \epsilon_t) + GPX_{t-1} + GQZ_t + HX_{t-1} + LNZ_t + MZ_t\} \\
&FP^2X_{t-1} + FPQZ_t + FNQZ_t +GPX_{t-1} + GQZ_t + HX_{t-1} + LNZ_t + MZ_t \\
&[(FP + G)P + H]X_{t-1} + [Q(FP + G)+ M + N(FQ + L)]Z_t,
\end{align*}
as desired.

\section*{Perturbation Methods}

\subsection*{Exercise 1}
After taking derivatives and simplifying the terms, we end up with the following closed form:
$$x_{uuu} =\frac{ F_{xxx}x_u^3 + 3[F_{xx}x_u x_{uu} + F_{xu}x_{uu} + F_{xxu}x_u^2 + F_{xuu}x_u] + F_{uuu}}{F_x}$$


\end{document}